renamed some examples

aneris/examples/transactional_consistency/read_committed/examples/dirty_read/dirty_read_code.v
@@ -7,31 +7,15 @@ From aneris.examples.transactional_consistency.snapshot_isolation Require Import
 From aneris.examples.transactional_consistency.snapshot_isolation.util Require Import util_code.
 
 Definition transaction1 : val :=
-  λ: "cst",
-  start "cst";;
-  write "cst" #"x" #1;;
-  let: "vy" := read "cst" #"y" in
-  (if: "vy" = (SOME #1)
-   then  write "cst" #"a" #1
-   else  #());;
-  commitU "cst".
+  λ: "cst", start "cst";;
+             write "cst" #"x" #1;;
+             loop #().
 
 Definition transaction2 : val :=
   λ: "cst",
   start "cst";;
-  write "cst" #"y" #1;;
   let: "vx" := read "cst" #"x" in
-  (if: "vx" = (SOME #1)
-   then  write "cst" #"b" #1
-   else  #());;
-  commitU "cst".
-
-Definition transaction3 : val :=
-  λ: "cst",
-  start "cst";;
-  let: "va" := read "cst" #"a" in
-  let: "vb" := read "cst" #"b" in
-  assert: (~ (("va" = (SOME #1)) && ("vb" = (SOME #1))));;
+  assert: ("vx" = NONE);;
   commitU "cst".
 
 Definition transaction1_client : val :=
@@ -43,10 +27,5 @@ Definition transaction2_client : val :=
   λ: "caddr" "kvs_addr",
   let: "cst" := init_client_proxy int_serializer "caddr" "kvs_addr" in
   transaction2 "cst".
-
-Definition transaction3_client : val :=
-  λ: "caddr" "kvs_addr",
-  let: "cst" := init_client_proxy int_serializer "caddr" "kvs_addr" in
-  transaction3 "cst".
 
 Definition server : val := λ: "srv", init_server int_serializer "srv".
